Filesys/PathBasedFS.i.dfy
@@ -8,67 +8,67 @@ module PathBasedFS {
   import opened PathSpec
   import opened Options
 
-  type ValidMeta(==,!new) = m : MetaData | m.MetaData? witness InitRootMetaData()
-
-  datatype PathMeta =
-    | Empty
-    | PathMeta(m: ValidMeta, hidden: bool) // hidden used by hardlink
-    | RedirectMeta(source: Path) // used by hardlink
-
-  type MetaView = imap<Path, PathMeta>
+  type MetaView = imap<Path, MetaData>
   type DataView = imap<Path, Data>
 
-  datatype FileSys = FileSys(meta_map: MetaView, data_map: DataView)
+  datatype View = View(meta_map: MetaView, data_map: DataView)
+  datatype FileSys = FileSys(content: View, hidden: View)
+
+  predicate ViewComplete(v: View)
+  {
+    && (forall p :: p in v.meta_map && p in v.data_map)
+  }
 
   predicate WF(fs: FileSys)
   {
-    && (forall p :: p in fs.meta_map && p in fs.data_map)
+    && ViewComplete(fs.content)
+    && ViewComplete(fs.hidden)
   }
 
   predicate PathExists(fs: FileSys, path: Path)
   requires WF(fs)
   {
-    var m := fs.meta_map[path];
-    || (m.PathMeta? && !m.hidden)
-    || m.RedirectMeta?
+    && !fs.content.meta_map[path].EmptyMeta?
   }
 
   predicate Init(fs: FileSys)
   {
-    var empty_meta := imap p :: Empty;
-    && fs.meta_map == empty_meta[RootDir := PathMeta(InitRootMetaData(), false)]
-    && fs.data_map == (imap id :: EmptyData())
+    var empty_meta := imap p :: EmptyMeta;
+    var empty_data := imap p :: EmptyData();
+
+    && fs.content.meta_map == empty_meta[RootDir := InitRootMetaData()]
+    && fs.content.data_map == empty_data
+    && fs.hidden.meta_map == empty_meta
+    && fs.hidden.data_map == empty_data
   }
 
   /// Inv conditions
 
-  function GetMeta(fs: FileSys, path: Path) : PathMeta
+  function GetMeta(fs: FileSys, path: Path) : MetaData
   requires WF(fs)
   {
-    var m := fs.meta_map[path];
-    if m.RedirectMeta? then fs.meta_map[m.source] else m
+    var m := fs.content.meta_map[path];
+    if m.RedirectMeta? then fs.hidden.meta_map[m.source] else m
   }
 
-  // I want to write this based on the source stuff
   function AliasPaths(fs: FileSys, path: Path) : (aliases: iset<Path>)
   requires WF(fs)
-  requires fs.meta_map[path].RedirectMeta?
+  requires fs.content.meta_map[path].RedirectMeta?
   ensures forall p :: p in aliases <==> (
-    && fs.meta_map[p].RedirectMeta? 
-    && fs.meta_map[p].source == fs.meta_map[path].source)
+    && fs.content.meta_map[p].RedirectMeta? 
+    && fs.content.meta_map[p].source == fs.content.meta_map[path].source)
   {
-    var src := fs.meta_map[path].source;
-    iset p | fs.meta_map[p].RedirectMeta? && fs.meta_map[p].source == src
+    var src := fs.content.meta_map[path].source;
+    iset p | fs.content.meta_map[p].RedirectMeta? && fs.content.meta_map[p].source == src
   }
 
   predicate NoAlias(fs: FileSys, path: Path)
   requires WF(fs)
   {
-    || fs.meta_map[path].PathMeta?
-    || (fs.meta_map[path].RedirectMeta? ==> AliasPaths(fs, path) == iset{path})
+    && (fs.content.meta_map[path].RedirectMeta? ==> AliasPaths(fs, path) == iset{path})
   }
 
-  // predicate DirImpliesHasNoAlias(fs: FileSys, path: Path)
+  // predicate DirImpliesNoAlias(fs: FileSys, path: Path)
   // requires WF(fs)
   // requires PathExists(fs, path)
   // {
@@ -80,39 +80,45 @@ module PathBasedFS {
   {
     var parent_dir := GetParentDir(path);
     && PathExists(fs, parent_dir)
-    && GetMeta(fs, parent_dir).PathMeta?
-    && GetMeta(fs, parent_dir).m.ftype.Directory?
+    && GetMeta(fs, parent_dir).MetaData?
+    && GetMeta(fs, parent_dir).ftype.Directory?
   }
 
   predicate ValidNewPath(fs: FileSys, path: Path)
   requires WF(fs)
   {
     && ParentDirIsDir(fs, path)
-    && fs.meta_map[path].Empty?
+    && fs.content.meta_map[path].EmptyMeta?
+  }
+
+  predicate ValidNewHiddenName(fs: FileSys, path: Option<Path>)
+  requires WF(fs)
+  {
+    && (path.Some? ==> fs.hidden.meta_map[path.value].EmptyMeta?)
   }
 
   predicate ValidNewId(fs: FileSys, id: ID)
   requires WF(fs)
   {
     && id.ID?
-    && (forall p | fs.meta_map[p].PathMeta? :: fs.meta_map[p].m.id != id)
+    && (forall p | fs.content.meta_map[p].MetaData? :: fs.content.meta_map[p].id != id)
+    && (forall p | fs.hidden.meta_map[p].MetaData? :: fs.hidden.meta_map[p].id != id)
   }
 
   predicate IsEmptyDir(fs: FileSys, dir: Path)
   requires WF(fs)
   {
-    && (forall k | BeneathDir(dir, k) :: fs.meta_map[k].Empty?)
+    && (forall k | IsDirEntry(dir, k) :: fs.content.meta_map[k].EmptyMeta?)
   }
 
   /// FileSys Ops
 
-  predicate GetAttr(fs: FileSys, fs':FileSys, path: Path, attr: ValidMeta)
+  predicate GetAttr(fs: FileSys, fs':FileSys, path: Path, attr: MetaData)
   {
     && WF(fs)
     && PathExists(fs, path)
     && fs' == fs
-    && GetMeta(fs, path).PathMeta?
-    && attr == GetMeta(fs, path).m
+    && attr == GetMeta(fs, path)
   }
 
   predicate ReadLink(fs: FileSys, fs':FileSys, path: Path, link_path: Path)
@@ -120,17 +126,23 @@ module PathBasedFS {
     && WF(fs)
     && PathExists(fs, path)
     && fs' == fs
-    && GetMeta(fs, path).PathMeta?
-    && GetMeta(fs, path).m.ftype.SymLink?
-    && link_path == GetMeta(fs, path).m.ftype.source
+    && GetMeta(fs, path).MetaData?
+    && GetMeta(fs, path).ftype.SymLink?
+    && link_path == GetMeta(fs, path).ftype.source
   }
 
-  function UpdatePathTime(fs: FileSys, path: Path, time: Time) : PathMeta
-  requires WF(fs)
+  function MetaDataUpdateTime(m: MetaData, atime: Time, mtime: Time, ctime: Time): MetaData
+  requires m.MetaData?
   {
-    var m := GetMeta(fs, path);
-    if m.PathMeta? 
-    then PathMeta(MetaDataUpdateTime(m.m, m.m.atime, time, time), m.hidden)
+    MetaData(m.id, m.ftype, m.perm, m.uid, m.gid, atime, mtime, ctime)
+  }
+
+  function UpdatePathTime(v: View, path: Path, time: Time) : MetaData
+  requires ViewComplete(v)
+  {
+    var m := v.meta_map[path];
+    if m.MetaData? 
+    then MetaDataUpdateTime(m, m.atime, time, time)
     else m
   }
 
@@ -141,35 +153,37 @@ module PathBasedFS {
     && ValidNewPath(fs, path)
     && ValidNewMetaData(m, path)
     && ValidNewId(fs, m.id)
-    // Entry Not Present
-    && fs.meta_map[path].Empty?
-    && fs.data_map[path] == EmptyData()
     // Updated maps
     && var parent_dir := GetParentDir(path);
-    && var parent_m' := UpdatePathTime(fs, parent_dir, m.mtime);
-    && fs'.meta_map == fs.meta_map[parent_dir := parent_m'][path := PathMeta(m, false)]
-    && fs'.data_map == fs.data_map
+    && var parent_m' := UpdatePathTime(fs.content, parent_dir, m.mtime);
+    && fs'.content.meta_map == fs.content.meta_map[parent_dir := parent_m'][path := m]
+    && fs'.content.data_map == fs.content.data_map
+    && fs'.hidden == fs.hidden
   }
 
-  function UpdatePathCtime(fs: FileSys, path: Path, time: Time) : PathMeta
-  requires WF(fs)
+  function UpdatePathCtime(v: View, path: Path, time: Time) : MetaData
+  requires ViewComplete(v)
   {
-    var m := GetMeta(fs, path);
-    if m.PathMeta? 
-    then PathMeta(MetaDataUpdateTime(m.m, m.m.atime, m.m.mtime, time), m.hidden)
+    var m := v.meta_map[path];
+    if m.MetaData? 
+    then MetaDataUpdateTime(m, m.atime, m.mtime, time)
     else m
   }
 
-  function MetaDataDelete(fs: FileSys, path: Path, ctime: Time): PathMeta
+  function HiddenMetaDataDelete(fs: FileSys, path: Path, ctime: Time): MetaData
   requires WF(fs)
+  requires fs.content.meta_map[path].RedirectMeta?
   {
-    if NoAlias(fs, path) then Empty else UpdatePathCtime(fs, path, ctime)
+    var m := fs.content.meta_map[path];
+    if NoAlias(fs, path) then EmptyMeta else UpdatePathCtime(fs.hidden, m.source, ctime)
   }
 
-  function DataDelete(fs: FileSys, path: Path): Data
+  function HiddenDataDelete(fs: FileSys, path: Path): Data
   requires WF(fs)
+  requires fs.content.meta_map[path].RedirectMeta?
   {
-    if NoAlias(fs, path) then EmptyData() else fs.data_map[path]
+    var m := fs.content.meta_map[path];
+    if NoAlias(fs, path) then EmptyData() else fs.hidden.data_map[m.source]
   }
 
   predicate Delete(fs: FileSys, fs':FileSys, path: Path, ctime: Time)
@@ -178,76 +192,70 @@ module PathBasedFS {
     && WF(fs')
     && path != RootDir
     && PathExists(fs, path)
-    && var m := fs.meta_map[path];
-    && (m.PathMeta? && m.m.ftype.Directory? ==> IsEmptyDir(fs, path))
+    && var m := fs.content.meta_map[path];
+    && (m.MetaData? && m.ftype.Directory? ==> IsEmptyDir(fs, path))
     // maps after delete
     && var parent_dir := GetParentDir(path);
-    && var parent_m' := UpdatePathCtime(fs, parent_dir, ctime);
-    && (m.PathMeta? ==> fs'.meta_map == fs.meta_map[path := Empty][parent_dir := parent_m'])
-    && (m.RedirectMeta? ==> fs'.meta_map == fs.meta_map[path := Empty]
-          [m.source := MetaDataDelete(fs, path, ctime)][parent_dir := parent_m'])
-    && fs'.data_map == fs.data_map[path := DataDelete(fs, path)]
+    && var parent_m' := UpdatePathCtime(fs.content, parent_dir, ctime);
+    && fs'.content.meta_map == fs.content.meta_map[path := EmptyMeta][parent_dir := parent_m']
+    && fs'.content.data_map == fs.content.data_map[path := EmptyData()]
+    && (m.MetaData? ==> fs'.hidden == fs.hidden)
+    && (m.RedirectMeta? ==>
+      // need to clean up hidden file if this 
+      && fs'.hidden.meta_map == fs.hidden.meta_map[m.source := HiddenMetaDataDelete(fs, path, ctime)]
+      && fs'.hidden.data_map == fs.hidden.data_map[m.source := HiddenDataDelete(fs, path)])
   }
 
-  function MetaMapRename(fs: FileSys, src: Path, dst: Path, ctime: Time): (meta_map: MetaView)
-  requires WF(fs)
+  function MetaMapRename(v: View, src: Path, dst: Path, ctime: Time): (meta_map: MetaView)
+  requires ViewComplete(v)
   {
     imap path ::
-      if path == src || BeneathDir(src, path) then Empty
-      else if path == dst then UpdatePathCtime(fs, src, ctime)
-      else if BeneathDir(dst, path) then (
-        var suffix := path[|dst|..];
-        fs.meta_map[src + suffix]
-      ) else if fs.meta_map[dst].RedirectMeta? && fs.meta_map[dst].source == path then (
-        UpdatePathCtime(fs, dst, ctime)
-      ) else if path == GetParentDir(src) || path == GetParentDir(dst) then (
-        UpdatePathTime(fs, path, ctime)
-      ) else (
-        fs.meta_map[path]
-      )
+      if path == src || BeneathDir(src, path) then EmptyMeta // clear all valid source entries
+      else if path == dst then UpdatePathCtime(v, src, ctime) // update src ctime if not hidden
+      else if BeneathDir(dst, path) then v.meta_map[src + path[|dst|..]] // redirect dst to src prefix
+      else if path == GetParentDir(src) || path == GetParentDir(dst) then UpdatePathTime(v, path, ctime) // update parentdir
+      else v.meta_map[path]
   }
 
-  function DataMapRename(fs: FileSys, src: Path, dst: Path, ctime: Time): (data_map: DataView)
-  requires WF(fs)
+  function DataMapRename(v: View, src: Path, dst: Path, ctime: Time): (data_map: DataView)
+  requires ViewComplete(v)
   {
     imap path ::
       if path == src || BeneathDir(src, path) then EmptyData()
-      else if path == dst || BeneathDir(dst, path) then (
-        var suffix := path[|dst|..];
-        fs.data_map[src + suffix]
-      ) else if fs.meta_map[dst].RedirectMeta? && fs.meta_map[dst].source == path then (
-        DataDelete(fs, dst)
-      ) else (
-        fs.data_map[path]
-      )
+      else if path == dst || BeneathDir(dst, path) then v.data_map[src + path[|dst|..]]
+      else v.data_map[path]
   }
 
   predicate Rename(fs: FileSys, fs':FileSys, src: Path, dst: Path, ctime: Time)
   {
     && WF(fs)
     && WF(fs')
+    && src != RootDir
+    && src != dst
     && PathExists(fs, src)
-    && !BeneathDir(dst, src)
+    && !BeneathDir(src, dst)
     && (PathExists(fs, dst) || ValidNewPath(fs, dst))
-
-    && var src_m := GetMeta(fs, src);
+    // if dst exists and is a directory 
+    // dst needs to be empty and src has to be a directory too
+    && var src_m := fs.content.meta_map[src];
+    && var dst_m := fs.content.meta_map[dst];
     && (PathExists(fs, dst) ==>
-      && var dst_m := GetMeta(fs, dst);
-      && (src_m.PathMeta? && src_m.m.ftype.Directory?
-          <==> dst_m.PathMeta? && dst_m.m.ftype.Directory?)
-      && (dst_m.PathMeta? && dst_m.m.ftype.Directory?
-          ==> IsEmptyDir(fs, dst)))
-
-    && fs'.meta_map == MetaMapRename(fs, src, dst, ctime)
-    && fs'.data_map == DataMapRename(fs, src, dst, ctime)
+      && (src_m.MetaData? && src_m.ftype.Directory? <==> dst_m.MetaData? && dst_m.ftype.Directory?)
+      && (dst_m.MetaData? && dst_m.ftype.Directory? ==> IsEmptyDir(fs, dst)))
+    // updated maps
+    && fs'.content.meta_map == MetaMapRename(fs.content, src, dst, ctime)
+    && fs'.content.data_map == DataMapRename(fs.content, src, dst, ctime)
+    && (!dst_m.RedirectMeta? ==> fs'.hidden == fs.hidden)
+    && (dst_m.RedirectMeta? ==> 
+      && fs'.hidden.meta_map == fs.hidden.meta_map[dst_m.source := HiddenMetaDataDelete(fs, dst, ctime)]
+      && fs'.hidden.data_map == fs.hidden.data_map[dst_m.source := HiddenDataDelete(fs, dst)])
   }
 
-  function LinkMeta(fs: FileSys, path: Path, time: Time) : PathMeta
-  requires WF(fs)
+  function LinkMeta(v: View, path: Path, time: Time) : MetaData
+  requires ViewComplete(v)
   {
-    var m := GetMeta(fs, path);
-    if m.PathMeta? 
-    then PathMeta(MetaDataUpdateTime(m.m, m.m.atime, m.m.mtime, time), true)
+    var m := v.meta_map[path];
+    if m.MetaData? then MetaDataUpdateTime(m, m.atime, m.mtime, time)
     else m
   }
 
@@ -255,32 +263,28 @@ module PathBasedFS {
   {
     && WF(fs)
     && WF(fs')
-    // NOTE: won't work for hardlink other filesystem files
-    // robj: Hard-links can't cross file systems, so not a problem.
     && PathExists(fs, source)
     && ValidNewPath(fs, dest)
-    && var m := fs.meta_map[source];
-    && (m.PathMeta? ==> !m.m.ftype.Directory?)
-    && (m.PathMeta? <==> hiddenName.Some?) // generating an alias for the first time
-    && (hiddenName.Some? ==> fs.meta_map[hiddenName.value].Empty? && hiddenName.value != dest)
+    && ValidNewHiddenName(fs, hiddenName)
+    && var m := fs.content.meta_map[source];
+    && (m.MetaData? ==> !m.ftype.Directory? && hiddenName.Some?)
     // updated maps
     && var parent_dir := GetParentDir(dest);
-    && var parent_m' := UpdatePathTime(fs, parent_dir, ctime);
-    && var p := if m.RedirectMeta? then m.source else hiddenName.value;
-    && fs'.meta_map == fs.meta_map[parent_dir := parent_m']
-                        [p := LinkMeta(fs, source, ctime)]
-                        [source := RedirectMeta(p)]
-                        [dest := RedirectMeta(p)]
-    && fs'.data_map == fs.data_map
+    && var parent_m' := UpdatePathTime(fs.content, parent_dir, ctime);
+    && var p := if m.MetaData? then hiddenName.value else m.source;
+    && fs'.content.meta_map == fs.content.meta_map[parent_dir := parent_m'][source := RedirectMeta(p)][dest := RedirectMeta(p)]
+    && fs'.content.data_map == fs.content.data_map[p := EmptyData()]
+    && (m.MetaData? ==> 
+      && fs'.hidden.meta_map == fs.hidden.meta_map[hiddenName.value := LinkMeta(fs.content, source, ctime)]
+      && fs'.hidden.data_map == fs.hidden.data_map[hiddenName.value := fs.content.data_map[source]])
+    && (m.RedirectMeta? ==> fs'.hidden == fs.hidden)
   }
 
-  function MetaDataChangeAttr(fs: FileSys, path: Path, perm: int, uid:int, gid: int, ctime: Time): PathMeta
-  requires WF(fs)
-  requires PathExists(fs, path)
+  function MetaDataChangeAttr(v: View, path: Path, perm: int, uid:int, gid: int, ctime: Time): MetaData
+  requires ViewComplete(v)
   {
-    var m := GetMeta(fs, path);
-    if m.PathMeta? 
-    then PathMeta(MetaData(m.m.id, m.m.ftype, perm, uid, gid, m.m.atime, m.m.mtime, ctime), m.hidden)
+    var m := v.meta_map[path];
+    if m.MetaData? then MetaData(m.id, m.ftype, perm, uid, gid, m.atime, m.mtime, ctime)
     else m
   }
 
@@ -291,14 +295,18 @@ module PathBasedFS {
     && WF(fs')
     && PathExists(fs, path)
     // updated maps
-    && var p := if fs.meta_map[path].PathMeta? then path else fs.meta_map[path].source;
-    && fs'.meta_map == fs.meta_map[p := MetaDataChangeAttr(fs, path, perm, uid, gid, ctime)]
-    && fs'.data_map == fs.data_map
-  }
-
-  function MetaDataUpdateTime(m: ValidMeta, atime: Time, mtime: Time, ctime: Time): ValidMeta
-  {
-    MetaData(m.id, m.ftype, m.perm, m.uid, m.gid, atime, mtime, ctime)
+    && var m := fs.content.meta_map[path];
+    && var p := if m.MetaData? then path else m.source;
+    && var v := if m.MetaData? then fs.content else fs.hidden;
+    && var m' := MetaDataChangeAttr(v, p, perm, uid, gid, ctime);
+    && (m.MetaData? ==> 
+      && fs'.content.meta_map == fs.content.meta_map[p := m']
+      && fs'.content.data_map == fs.content.data_map
+      && fs'.hidden == fs.hidden)
+    && (m.RedirectMeta? ==> 
+      && fs'.content == fs.content
+      && fs'.hidden.meta_map == fs.hidden.meta_map[p := m']
+      && fs'.hidden.data_map == fs.hidden.data_map)
   }
 
   function ZeroData(size: nat) : (d: Data) { seq(size, i => 0) }
@@ -316,12 +324,23 @@ module PathBasedFS {
     && WF(fs')
     && 0 <= size
     && PathExists(fs, path)
-    && var m := GetMeta(fs, path);
-    && m.PathMeta? && m.m.ftype.File?
+    && GetMeta(fs, path).MetaData?
+    && GetMeta(fs, path).ftype.File?
     // updated maps
-    && var p := if fs.meta_map[path].PathMeta? then path else fs.meta_map[path].source;
-    && fs'.meta_map == fs.meta_map[p := UpdatePathTime(fs, path, time)]
-    && fs'.data_map == fs.data_map[p := DataTruncate(fs.data_map[p], size)]
+    && var m := fs.content.meta_map[path];
+    && var p := if m.MetaData? then path else m.source;
+    && var v := if m.MetaData? then fs.content else fs.hidden;
+    && var d := if m.MetaData? then fs.content.data_map[p] else fs.hidden.data_map[p];
+    && var m' := UpdatePathTime(v, p, time);
+
+    && (m.MetaData? ==>
+      && fs'.content.meta_map == fs.content.meta_map[p := m']
+      && fs'.content.data_map == fs.content.data_map[p := DataTruncate(d, size)]
+      && fs'.hidden == fs.hidden)
+    && (m.RedirectMeta? ==>
+      && fs'.content == fs.content
+      && fs'.hidden.meta_map == fs.hidden.meta_map[p := m']
+      && fs'.hidden.data_map == fs.hidden.data_map[p := DataTruncate(d, size)])
   }
 
   predicate Read(fs: FileSys, fs':FileSys, path: Path, offset: int, size: int, data: Data)
@@ -329,11 +348,11 @@ module PathBasedFS {
     && WF(fs)
     && fs' == fs
     && PathExists(fs, path)
-    && var m := GetMeta(fs, path);
-    && (m.PathMeta? ==> m.m.ftype.File?)
-    && var p := if fs.meta_map[path].PathMeta? then path else fs.meta_map[path].source;
-    && 0 <= offset <= offset+size <= |fs.data_map[p]|
-    && data == fs.data_map[p][offset..offset+size]
+    && (GetMeta(fs, path).MetaData? ==> GetMeta(fs, path).ftype.File?)
+    && var m := fs.content.meta_map[path];
+    && var d := if m.MetaData? then fs.content.data_map[path] else fs.hidden.data_map[m.source];
+    && 0 <= offset <= offset+size <= |d|
+    && data == d[offset..offset+size]
   }
 
   function DataWrite(d: Data, data: Data, offset: int, size: int): (d': Data)
@@ -345,12 +364,11 @@ module PathBasedFS {
     if offset+size > |d| then d[..offset] + data else d[..offset] + data + d[offset+size..]
   }
 
-  function UpdatePathWriteTime(fs: FileSys, path: Path, time: Time) : PathMeta
-  requires WF(fs)
+  function UpdatePathWriteTime(v: View, path: Path, time: Time) : MetaData
+  requires ViewComplete(v)
   {
-    var m := GetMeta(fs, path);
-    if m.PathMeta? 
-    then PathMeta(MetaDataUpdateTime(m.m, time, time, time), m.hidden)
+    var m := v.meta_map[path];
+    if m.MetaData? then MetaDataUpdateTime(m, time, time, time)
     else m
   }
 
@@ -360,21 +378,29 @@ module PathBasedFS {
     && WF(fs')
     && PathExists(fs, path)
     && |data| == size
-    && var m := GetMeta(fs, path);
-    && (m.PathMeta? ==> m.m.ftype.File?)
-    && var p := if fs.meta_map[path].PathMeta? then path else fs.meta_map[path].source;
-    && 0 <= offset <= |fs.data_map[p]|
-    // updated maps
-    && fs'.meta_map == fs.meta_map[p := UpdatePathWriteTime(fs, path, time)]
-    && fs'.data_map == fs.data_map[p := DataWrite(fs.data_map[p], data, offset, size)]
+    && (GetMeta(fs, path).MetaData? ==> GetMeta(fs, path).ftype.File?)
+    && var m := fs.content.meta_map[path];
+    && var v := if m.MetaData? then fs.content else fs.hidden;
+    && var p := if m.MetaData? then path else m.source;
+    && var d := if m.MetaData? then fs.content.data_map[p] else fs.hidden.data_map[p];
+    && 0 <= offset <= |d|
+    && var m' := UpdatePathWriteTime(v, p, time);
+    && var d' := DataWrite(d, data, offset, size);
+    && (m.MetaData? ==> 
+      && fs'.content.meta_map == fs.content.meta_map[p := m']
+      && fs'.content.data_map == fs.content.data_map[p := d']
+      && fs'.hidden == fs.hidden)
+    && (m.RedirectMeta? ==>
+      && fs'.content == fs.content
+      && fs'.hidden.meta_map == fs.hidden.meta_map[p := m']
+      && fs'.hidden.data_map == fs.hidden.data_map[p := d'])
   }
 
-  function UpdatePathUpdateTime(fs: FileSys, path: Path, atime: Time, mtime: Time, ctime: Time) : PathMeta
-  requires WF(fs)
+  function UpdatePathUpdateTime(v: View, path: Path, atime: Time, mtime: Time, ctime: Time) : MetaData
+  requires ViewComplete(v)
   {
-    var m := GetMeta(fs, path);
-    if m.PathMeta? 
-    then PathMeta(MetaDataUpdateTime(m.m, atime, mtime, ctime), m.hidden)
+    var m := v.meta_map[path];
+    if m.MetaData? then MetaDataUpdateTime(m, atime, mtime, ctime)
     else m
   }
 
@@ -383,9 +409,19 @@ module PathBasedFS {
     && WF(fs)
     && WF(fs')
     && PathExists(fs, path)
-    && var p := if fs.meta_map[path].PathMeta? then path else fs.meta_map[path].source;
-    && fs'.meta_map == fs.meta_map[p := UpdatePathUpdateTime(fs, path, atime, mtime, ctime)]
-    && fs'.data_map == fs.data_map
+    && var m := fs.content.meta_map[path];
+    && var v := if m.MetaData? then fs.content else fs.hidden;
+    && var p := if m.MetaData? then path else m.source;
+    && var m' := UpdatePathUpdateTime(v, p, atime, mtime, ctime);
+    // updated maps
+    && (m.MetaData? ==> 
+      && fs'.content.meta_map == fs.content.meta_map[p := m']
+      && fs'.content.data_map == fs.content.data_map
+      && fs'.hidden == fs.hidden)
+    && (m.RedirectMeta? ==> 
+      && fs'.content == fs.content
+      && fs'.hidden.meta_map == fs.hidden.meta_map[p := m']
+      && fs'.hidden.data_map == fs.hidden.data_map)
   }
 
   predicate ValidDirEntry(fs: FileSys, de: DirEntry)
@@ -393,18 +429,17 @@ module PathBasedFS {
   {
     && PathExists(fs, de.path)
     && var m := GetMeta(fs, de.path);
-    && (m.PathMeta? ==> 
-      && de.id == m.m.id
-      && de.ftype == m.m.ftype)
+    && (m.MetaData? ==>
+      && de.id == m.id
+      && de.ftype == m.ftype)
   }
 
   predicate ReadDir(fs: FileSys, fs':FileSys, dir: Path, start: Option<Path>, results: seq<DirEntry>, done: bool)
   {
     && WF(fs)
     && fs' == fs
-    && PathExists(fs, dir)
-    && fs.meta_map[dir].PathMeta?
-    && fs.meta_map[dir].m.ftype.Directory?
+    && fs.content.meta_map[dir].MetaData?
+    && fs.content.meta_map[dir].ftype.Directory?
     && (start.Some? ==> IsDirEntry(dir, start.value))
     // results actually belong to this directory
     && (forall i | 0 <= i < |results| :: IsDirEntry(dir, results[i].path))
@@ -432,7 +467,7 @@ module PathBasedFS {
   }
 
   datatype Step =
-    | GetAttrStep(path: Path, attr: ValidMeta)
+    | GetAttrStep(path: Path, attr: MetaData)
     | ReadLinkStep(path: Path, link_path: Path)
     | CreateStep(path: Path, m: MetaData) // mknod, mkdir, symlink
     | DeleteStep(path: Path, ctime: Time) // unlink and rmdir
