Filesys/PathBasedFSInv.i.dfy
@@ -8,16 +8,22 @@ module PathBasedFSInv {
   import opened FSTypes
   import opened PathSpec
 
+  // redirect meta should have no corresponding data entry ==> emptydata
+
   predicate Inv(fs: FileSys)
   {
     && WF(fs)
+    // consistency of hidden map
+    // && (forall p | fs.hidden.meta_map[p].)
+
+
     // path is connected
-    && (forall path | PathExists(fs, path) && path != RootDir :: ParentDirIsDir(fs, path))
+    // && (forall path | PathExists(fs, path) && path != RootDir :: ParentDirIsDir(fs, path))
     // redirect meta points to a valid and hidden path meta
-    && (forall path | fs.meta_map[path].RedirectMeta? :: 
-        && fs.meta_map[fs.meta_map[path].source].PathMeta?
-        && fs.meta_map[fs.meta_map[path].source].hidden
-        && !fs.meta_map[fs.meta_map[path].source].m.ftype.Directory?)
+    // && (forall path | fs.meta_map[path].RedirectMeta? :: 
+    //     && fs.meta_map[fs.meta_map[path].source].PathMeta?
+    //     && fs.meta_map[fs.meta_map[path].source].hidden
+    //     && !fs.meta_map[fs.meta_map[path].source].m.ftype.Directory?)
   }
 
   lemma InitImpliesInv(fs: FileSys)
@@ -26,165 +32,255 @@ module PathBasedFSInv {
   {
   }
 
-  lemma NextPreservesInv(fs: FileSys, fs': FileSys)
-  requires Inv(fs)
-  requires Next(fs, fs')
-  ensures Inv(fs')
-  {
-    var step :| NextStep(fs, fs', step);
-    NextStepPreservesInv(fs, fs', step);
-  }
-
-  lemma NextStepPreservesInv(fs: FileSys, fs': FileSys, step: Step)
-  requires Inv(fs)
-  requires NextStep(fs, fs', step)
-  ensures Inv(fs')
-  {
-    match step {
-      case DeleteStep(path, ctime) => DeletePreservesInv(fs, fs', path, ctime);
-      case RenameStep(source, dest, ctime) => RenamePreservesInv(fs, fs', source, dest, ctime);
-      case LinkStep(source, dest, ctime, hiddenName) => LinkPreservesInv(fs, fs', source, dest, ctime, hiddenName);
-      case _ => {
-        if step.CreateStep? || step.ChangeAttrStep? || step.TruncateStep? || step.WriteStep? || step.UpdateTimeStep? {
-          SimpleStepPreservesInv(fs, fs', step);
-        }
-      }
-    }
-  }
-
-  lemma DeletePreservesInv(fs: FileSys, fs': FileSys, path: Path, ctime: Time)
-  requires Inv(fs)
-  requires Delete(fs, fs', path, ctime)
-  ensures Inv(fs')
-  {
-    forall p | PathExists(fs', p) && p != RootDir
-    ensures ParentDirIsDir(fs', p)
-    {
-      assert PathExists(fs, p); // observe
-    }
-
-    // forall p | fs'.meta_map[p].RedirectMeta? 
-    // ensures fs'.meta_map[fs'.meta_map[p].source].PathMeta?
-    // ensures fs'.meta_map[fs'.meta_map[p].source].hidden
-    // ensures !fs'.meta_map[fs'.meta_map[p].source].m.ftype.Directory?
-    // {
-    //   var m := fs.meta_map[path];
-
-    //   if m.RedirectMeta? && fs'.meta_map[p].source == m.source {
-    //     assert fs.meta_map[p] == fs'.meta_map[p];
-    //     assert fs'.meta_map[m.source] == MetaDataDelete(fs, path, ctime);
-
-    //     if NoAlias(fs, path) {
-    //       assert p != path;
-    //       assert false;
-    //     }
-    //   }
-    // }
-    assert Inv(fs');
-  }
-
-  // lemma RenamedPathsRemainDifferent(src: Path, dst: Path, p1: Path, p2: Path)
-  // requires p1 != p2
-  // requires p1 == dst || BeneathDir(dst, p1)
-  // requires p2 == dst || BeneathDir(dst, p2)
-  // ensures src + p1[|dst|..] != src + p2[|dst|..]
+  // lemma NextPreservesInv(fs: FileSys, fs': FileSys)
+  // requires Inv(fs)
+  // requires Next(fs, fs')
+  // ensures Inv(fs')
   // {
-  //   if BeneathDir(dst, p1) && BeneathDir(dst, p2) {
-  //     assert p1[|dst|..] != p2[|dst|..];
+  //   var step :| NextStep(fs, fs', step);
+  //   NextStepPreservesInv(fs, fs', step);
+  // }
 
-  //     var p1' := src + p1[|dst|..];
-  //     var p2' := src + p2[|dst|..];
-
-  //     assert p1'[..|src|] == p2'[..|src|];
+  // lemma NextStepPreservesInv(fs: FileSys, fs': FileSys, step: Step)
+  // requires Inv(fs)
+  // requires NextStep(fs, fs', step)
+  // ensures Inv(fs')
+  // {
+  //   match step {
+  //     case DeleteStep(path, ctime) => DeletePreservesInv(fs, fs', path, ctime);
+  //     case RenameStep(source, dest, ctime) => RenamePreservesInv(fs, fs', source, dest, ctime);
+  //     case LinkStep(source, dest, ctime, hiddenName) => LinkPreservesInv(fs, fs', source, dest, ctime, hiddenName);
+  //     case _ => {
+  //       if step.CreateStep? || step.ChangeAttrStep? || step.TruncateStep? || step.WriteStep? || step.UpdateTimeStep? {
+  //         SimpleStepPreservesInv(fs, fs', step);
+  //       }
+  //     }
   //   }
   // }
 
-  lemma {:timeLimitMultiplier 2} RenamePreservesInv(fs: FileSys, fs': FileSys, src: Path, dst: Path, ctime: Time)
-  requires Inv(fs)
-  requires Rename(fs, fs', src, dst, ctime)
-  ensures Inv(fs')
-  {
-    forall p | PathExists(fs', p) && p != RootDir
-    ensures ParentDirIsDir(fs', p)
-    {
-      if p == dst {
-        assert ParentDirIsDir(fs', p);
-      } else if BeneathDir(dst, p) {
-        var parent_dir := GetParentDir(p);
-        var srcpath := src + p[|dst|..];
-        var srcparent_dir := GetParentDir(srcpath);
-        assert ParentDirIsDir(fs, srcpath); // observe
-        assert parent_dir == dst || BeneathDir(dst, parent_dir); // observe
+  // lemma DeletePreservesInv(fs: FileSys, fs': FileSys, path: Path, ctime: Time)
+  // requires Inv(fs)
+  // requires Delete(fs, fs', path, ctime)
+  // ensures Inv(fs')
+  // {
+  //   forall p | PathExists(fs', p) && p != RootDir
+  //   ensures ParentDirIsDir(fs', p)
+  //   {
+  //     assert PathExists(fs, p); // observe
+  //   }
 
-        if parent_dir == dst {
-          assert fs'.meta_map[parent_dir] == UpdatePathCtime(fs, src, ctime);
-        } else {
-          assert src + parent_dir[|dst|..] == srcparent_dir; // observe
-          assert fs'.meta_map[parent_dir] == fs.meta_map[srcparent_dir];
-        }
-      } else if fs.meta_map[dst].RedirectMeta? && fs.meta_map[dst].source == p {
-        assert ParentDirIsDir(fs', p);
-      } else if  p == GetParentDir(src) || p == GetParentDir(dst) {
-        assert ParentDirIsDir(fs', p);
-      } else {
-        assert ParentDirIsDir(fs, p);
-        assert ParentDirIsDir(fs', p);
-      }
-    }
+  //   // forall p | fs'.meta_map[p].RedirectMeta? 
+  //   // ensures fs'.meta_map[fs'.meta_map[p].source].PathMeta?
+  //   // ensures fs'.meta_map[fs'.meta_map[p].source].hidden
+  //   // ensures !fs'.meta_map[fs'.meta_map[p].source].m.ftype.Directory?
+  //   // {
+  //   //   var m := fs.meta_map[path];
 
-    forall p | fs'.meta_map[p].RedirectMeta? 
-    ensures fs'.meta_map[fs'.meta_map[p].source].PathMeta?
-    ensures fs'.meta_map[fs'.meta_map[p].source].hidden
-    ensures !fs'.meta_map[fs'.meta_map[p].source].m.ftype.Directory?
-    {
-      assume false;
-      // if (p == dest || p == source) && fs.meta_map[source].PathMeta? {
-      //   assert fs'.meta_map[hiddenName.value] == LinkMeta(fs, source, ctime);
-      // }
-    }
-    assert Inv(fs');
-  }
+  //   //   if m.RedirectMeta? && fs'.meta_map[p].source == m.source {
+  //   //     assert fs.meta_map[p] == fs'.meta_map[p];
+  //   //     assert fs'.meta_map[m.source] == MetaDataDelete(fs, path, ctime);
 
-  lemma LinkPreservesInv(fs: FileSys, fs': FileSys, source: Path, dest: Path, ctime: Time, hiddenName: Option<Path>)
-  requires Inv(fs)
-  requires Link(fs, fs', source, dest, ctime, hiddenName)
-  ensures Inv(fs')
-  {
-    forall p | PathExists(fs', p) && p != RootDir
-    ensures ParentDirIsDir(fs', p)
-    {
-      if p == dest {
-        assert ParentDirIsDir(fs', p);
-      } else {
-        assert PathExists(fs, p); // observe
-      }
-    }
+  //   //     if NoAlias(fs, path) {
+  //   //       assert p != path;
+  //   //       assert false;
+  //   //     }
+  //   //   }
+  //   // }
+  //   assert Inv(fs');
+  // }
 
-    forall p | fs'.meta_map[p].RedirectMeta? 
-    ensures fs'.meta_map[fs'.meta_map[p].source].PathMeta?
-    ensures fs'.meta_map[fs'.meta_map[p].source].hidden
-    ensures !fs'.meta_map[fs'.meta_map[p].source].m.ftype.Directory?
-    {
-      if (p == dest || p == source) && fs.meta_map[source].PathMeta? {
-        assert fs'.meta_map[hiddenName.value] == LinkMeta(fs, source, ctime);
-      }
-    }
-    assert Inv(fs');
-  }
+  // // lemma RenamedPathsRemainDifferent(src: Path, dst: Path, p1: Path, p2: Path)
+  // // requires p1 != p2
+  // // requires p1 == dst || BeneathDir(dst, p1)
+  // // requires p2 == dst || BeneathDir(dst, p2)
+  // // ensures src + p1[|dst|..] != src + p2[|dst|..]
+  // // {
+  // //   if BeneathDir(dst, p1) && BeneathDir(dst, p2) {
+  // //     assert p1[|dst|..] != p2[|dst|..];
 
-  lemma SimpleStepPreservesInv(fs: FileSys, fs': FileSys, step: Step)
-  requires Inv(fs)
-  requires NextStep(fs, fs', step)
-  requires step.CreateStep? || step.ChangeAttrStep? || step.TruncateStep? || step.WriteStep? || step.UpdateTimeStep?
-  ensures Inv(fs')
-  {
-    forall p | PathExists(fs', p) && p != RootDir 
-    ensures ParentDirIsDir(fs', p)
-    {
-      if p != step.path {
-        assert PathExists(fs, p); // observe
-      }
-    }
-    assert Inv(fs');
-  }
+  // //     var p1' := src + p1[|dst|..];
+  // //     var p2' := src + p2[|dst|..];
+
+  // //     assert p1'[..|src|] == p2'[..|src|];
+  // //   }
+  // // }
+
+  // lemma RenamePreservesInv(fs: FileSys, fs': FileSys, src: Path, dst: Path, ctime: Time)
+  // requires Inv(fs)
+  // requires Rename(fs, fs', src, dst, ctime)
+  // ensures Inv(fs')
+  // {
+  //   forall p | PathExists(fs', p) && p != RootDir
+  //   ensures ParentDirIsDir(fs', p)
+  //   {
+  //     if p == dst {
+  //       assert fs'.meta_map[p] == UpdatePathCtime(fs, src, ctime);
+  //       assert ParentDirIsDir(fs', dst);
+  //       // if PathExists(fs, dst) {
+  //       //   assert ParentDirIsDir(fs, dst);
+  //       //   assert ParentDirIsDir(fs', dst);
+  //       // } else {
+  //       //   assert ValidNewPath(fs, dst);
+  //       //   assert ParentDirIsDir(fs, dst);
+  //       //   assert GetParentDir(dst) != dst;
+  //       //   assert GetParentDir(src) != src;
+  //       //   assert fs'.meta_map[GetParentDir(dst)] == UpdatePathTime(fs, GetParentDir(dst), ctime);
+  //       //   assert ParentDirIsDir(fs', dst); // why?
+  //       // }
+  //       // assert ParentDirIsDir(fs', p);
+  //     } else if BeneathDir(dst, p) {
+  //       var srcpath := src + p[|dst|..];
+  //       assert PathExists(fs, srcpath);
+
+
+  //       // var parent_dir := GetParentDir(p);
+  //       //
+  //       // assert ParentDirIsDir(fs, srcpath); // observe
+  //       // assert src + parent_dir[|dst|..] == GetParentDir(srcpath); // observe
+  //       // assert parent_dir == dst || BeneathDir(dst, parent_dir); // observe
+  //       // assert fs'.meta_map[dst] == UpdatePathCtime(fs, src, ctime); // observe
+
+
+  //       assume ParentDirIsDir(fs', p);
+
+  //     } else {
+  //       assert PathExists(fs, p); // observe
+  //       // assert ParentDirIsDir(fs, p); // observe
+  //       // assert ParentDirIsDir(fs', p);
+  //     }
+  //   }
+
+
+
+  //   // forall p | PathExists(fs', p) && p != RootDir
+  //   // ensures ParentDirIsDir(fs', p)
+  //   // {
+  //   //   if p == dst {
+  //   //     assert fs'.meta_map[p] == UpdatePathCtime(fs, src, ctime);
+  //   //     assert ParentDirIsDir(fs', dst);
+  //   //     // if PathExists(fs, dst) {
+  //   //     //   assert ParentDirIsDir(fs, dst);
+  //   //     //   assert ParentDirIsDir(fs', dst);
+  //   //     // } else {
+  //   //     //   assert ValidNewPath(fs, dst);
+  //   //     //   assert ParentDirIsDir(fs, dst);
+  //   //     //   assert GetParentDir(dst) != dst;
+  //   //     //   assert GetParentDir(src) != src;
+  //   //     //   assert fs'.meta_map[GetParentDir(dst)] == UpdatePathTime(fs, GetParentDir(dst), ctime);
+  //   //     //   assert ParentDirIsDir(fs', dst); // why?
+  //   //     // }
+  //   //     // assert ParentDirIsDir(fs', p);
+  //   //   } else if BeneathDir(dst, p) {
+  //   //     var srcpath := src + p[|dst|..];
+  //   //     assert PathExists(fs, srcpath);
+
+
+  //   //     // var parent_dir := GetParentDir(p);
+  //   //     //
+  //   //     // assert ParentDirIsDir(fs, srcpath); // observe
+  //   //     // assert src + parent_dir[|dst|..] == GetParentDir(srcpath); // observe
+  //   //     // assert parent_dir == dst || BeneathDir(dst, parent_dir); // observe
+  //   //     // assert fs'.meta_map[dst] == UpdatePathCtime(fs, src, ctime); // observe
+
+
+  //   //     assume ParentDirIsDir(fs', p);
+
+  //   //   } else {
+  //   //     assert PathExists(fs, p); // observe
+  //   //     // assert ParentDirIsDir(fs, p); // observe
+  //   //     // assert ParentDirIsDir(fs', p);
+  //   //   }
+  //   // }
+
+  //   forall p | fs'.meta_map[p].RedirectMeta? 
+  //   ensures fs'.meta_map[fs'.meta_map[p].source].PathMeta?
+  //   ensures fs'.meta_map[fs'.meta_map[p].source].hidden
+  //   ensures !fs'.meta_map[fs'.meta_map[p].source].m.ftype.Directory?
+  //   {
+  //     // assert p != dst;
+  //     // assert p != src && !BeneathDir(src, p);
+
+  //     assume false;
+
+  //     // spec should skip hidden ones when moving things right?
+  //     // otherwise we would be 
+
+  //     // maybe we should have something that says we don't move the hidden name 
+
+
+  //     // if fs.meta_map[dst].RedirectMeta? && fs.meta_map[dst].source == p {
+  //     //   assume false;
+  //     // } else if p == GetParentDir(src) || p == GetParentDir(dst) {
+  //     //   // assume false;
+  //     // } else {
+
+  //     //   assume false;
+  //     // }
+
+  //     // imap path ::
+  //     // if path == src || BeneathDir(src, path) then Empty
+  //     // else if path == dst then UpdatePathCtime(fs, src, ctime)
+  //     // else if BeneathDir(dst, path) then (
+  //     //   var suffix := path[|dst|..];
+  //     //   fs.meta_map[src + suffix]
+  //     // ) else 
+      
+  //     // if fs.meta_map[dst].RedirectMeta? && fs.meta_map[dst].source == path then (
+  //     //   UpdatePathCtime(fs, dst, ctime)
+  //     // ) else if path == GetParentDir(src) || path == GetParentDir(dst) then (
+  //     //   UpdatePathTime(fs, path, ctime)
+  //     // ) else (
+  //     //   fs.meta_map[path]
+  //     // )
+
+  //     // assume false;
+  //     // if (p == dest || p == source) && fs.meta_map[source].PathMeta? {
+  //     //   assert fs'.meta_map[hiddenName.value] == LinkMeta(fs, source, ctime);
+  //     // }
+  //   }
+  //   assert Inv(fs');
+  // }
+
+  // lemma LinkPreservesInv(fs: FileSys, fs': FileSys, source: Path, dest: Path, ctime: Time, hiddenName: Option<Path>)
+  // requires Inv(fs)
+  // requires Link(fs, fs', source, dest, ctime, hiddenName)
+  // ensures Inv(fs')
+  // {
+  //   forall p | PathExists(fs', p) && p != RootDir
+  //   ensures ParentDirIsDir(fs', p)
+  //   {
+  //     if p == dest {
+  //       assert ParentDirIsDir(fs', p);
+  //     } else {
+  //       assert PathExists(fs, p); // observe
+  //     }
+  //   }
+
+  //   forall p | fs'.meta_map[p].RedirectMeta? 
+  //   ensures fs'.meta_map[fs'.meta_map[p].source].PathMeta?
+  //   ensures fs'.meta_map[fs'.meta_map[p].source].hidden
+  //   ensures !fs'.meta_map[fs'.meta_map[p].source].m.ftype.Directory?
+  //   {
+  //     if (p == dest || p == source) && fs.meta_map[source].PathMeta? {
+  //       assert fs'.meta_map[hiddenName.value] == LinkMeta(fs, source, ctime);
+  //     }
+  //   }
+  //   assert Inv(fs');
+  // }
+
+  // lemma SimpleStepPreservesInv(fs: FileSys, fs': FileSys, step: Step)
+  // requires Inv(fs)
+  // requires NextStep(fs, fs', step)
+  // requires step.CreateStep? || step.ChangeAttrStep? || step.TruncateStep? || step.WriteStep? || step.UpdateTimeStep?
+  // ensures Inv(fs')
+  // {
+  //   forall p | PathExists(fs', p) && p != RootDir 
+  //   ensures ParentDirIsDir(fs', p)
+  //   {
+  //     if p != step.path {
+  //       assert PathExists(fs, p); // observe
+  //     }
+  //   }
+  //   assert Inv(fs');
+  // }
 }
